Upgrade standard library

lib/crypto.fst
@@ -1,7 +1,6 @@
 module Crypto
-open Array
+open Bytes
 
-type bytes = seq<byte>
 type nbytes (n:nat) = b:bytes{length b == n} (* fixed-length bytes *)
 type tag = nbytes 20
 
@@ -15,20 +14,18 @@ assume val hmac_sha1_verify: hmac_key -> bytes -> tag -> Tot bool
 type block  = nbytes 32
 type cipher = nbytes (2 * 32)
 type aes_key = nbytes 16
+type aes_iv = nbytes 16
 
 assume val aes_128_keygen: unit -> Tot aes_key
 assume val aes_128_decrypt: aes_key -> cipher -> Tot block
 assume val aes_128_encrypt: k:aes_key -> p:block -> c:cipher {aes_128_decrypt k c = p}
 
-assume val aes_128_cbc_decrypt: aes_key -> bytes -> Tot bytes
-assume val aes_128_cbc_encrypt: k:aes_key -> p:bytes -> c:bytes {aes_128_cbc_decrypt k c = p}
+assume val aes_128_ivgen: unit -> Tot aes_iv
+assume val aes_128_cbc_decrypt: aes_key -> aes_iv -> bytes -> Tot bytes
+assume val aes_128_cbc_encrypt: k:aes_key -> iv:aes_iv -> p:bytes -> c:bytes {aes_128_cbc_decrypt k iv c = p}
 
-type rsakey = 
-     {modulus :  bytes;   
-      exponent:  bytes}
-
-type rsa_pkey = rsakey
-type rsa_skey = rsa_pkey * rsakey
+type rsa_pkey = {modulus: bytes; exponent: bytes}
+type rsa_skey = rsa_pkey * bytes
 
 assume val rsa_keygen: unit -> Tot rsa_skey
 assume val rsa_pk: rsa_skey -> Tot rsa_pkey
